Adjust base protocol and definitions.

examples/nsl_dh/impl.v
@@ -13,9 +13,9 @@ Unset Printing Implicit Defensive.
 
 (*
 
-A --> B: {g^a; nI; pkA}@pkB                         (msg1)
-B --> A: {g^a; g^b; nI; nR; pkB; N}@pkA             (msg2)
-A --> B: {g^a; g^b; pkA; nR}@pkB                     (msg3)
+A --> B: {g^a; pkA}@pkB                     (msg1)
+B --> A: {g^a; g^b; pkB; N}@pkA             (msg2)
+A --> B: {g^b; pkA}@pkB                     (msg3)
 
 Result: derive_key [pkA; pkB; g^a; g^b; g^ab]
 
@@ -30,39 +30,36 @@ Definition initiator : val := λ: "c" "skI" "pkR" "N",
   let: "pkI"  := pkey "skI" in
   let: "a"    := mk_nonce #() in
   let: "ga"   := mk_keyshare "a" in
-  let: "nI"   := mk_nonce #() in
   let: "m1"   := aenc "pkR" (Tag $ nsl_dhN.@"m1")
-                   (term_of_list ["ga"; "nI"; "pkI"]) in
+                   (term_of_list ["ga"; "pkI"]) in
   send "c" "m1";;
   bind: "m2"   := adec "skI" (Tag $ nsl_dhN.@"m2") (recv "c") in
   bind: "m2"   := list_of_term "m2" in
-  list_match: ["ga'"; "gb"; "nI'"; "nR"; "pkR'"; "N'"] := "m2" in
-  guard: eq_term "ga" "ga'" && eq_term "nI" "nI'" &&
+  list_match: ["ga'"; "gb"; "pkR'"; "N'"] := "m2" in
+  guard: eq_term "ga" "ga'" &&
          eq_term "pkR" "pkR'" && eq_term "N" "N'" in
   let: "gab"    := texp "gb" "a" in
   let: "secret" := term_of_list ["pkI"; "pkR"; "ga"; "gb"; "gab"] in
   let: "m3"     := aenc "pkR" (Tag $ nsl_dhN.@"m3")
-                     (term_of_list ["ga"; "gb"; "pkI"; "nR"]) in
+                     (term_of_list ["gb"; "pkI"]) in
   send "c" "m3";;
   SOME (derive_senc_key "secret").
 
-Definition resp : val := λ: "c" "skR" "N",
+Definition responder : val := λ: "c" "skR" "N",
   let: "pkR" := pkey "skR" in
   bind: "m1" := adec "skR" (Tag $ nsl_dhN.@"m1") (recv "c") in
   bind: "m1" := list_of_term "m1" in
-  list_match: ["ga"; "nI"; "pkI"] := "m1" in
+  list_match: ["ga"; "pkI"] := "m1" in
   guard: is_aenc_key "pkI" in
   let: "b"  := mk_nonce #() in
   let: "gb" := mk_keyshare "b" in
-  let: "nR" := mk_nonce #() in
   let: "m2" := aenc "pkI" (Tag $ nsl_dhN.@"m2")
-                 (term_of_list ["ga"; "gb"; "nI"; "nR"; "pkR"; "N"]) in
+                 (term_of_list ["ga"; "gb"; "pkR"; "N"]) in
   send "c" "m2";;
   bind: "m3" := adec "skR" (Tag $ nsl_dhN.@"m3") (recv "c") in
   bind: "m3" := list_of_term "m3" in
-  list_match: ["ga'"; "gb'"; "pkI'"; "nR'"] := "m3" in
-  guard: eq_term "ga" "ga'" && eq_term "gb" "gb'" &&
-         eq_term "pkI" "pkI'" && eq_term "nR" "nR'" in
+  list_match: ["gb'"; "pkI'"] := "m3" in
+  guard: eq_term "gb" "gb'" && eq_term "pkI" "pkI'" in
   let: "gab"    := texp "ga" "b" in
   let: "secret" := term_of_list ["pkI"; "pkR"; "ga"; "gb"; "gab"] in
   SOME ("pkI", derive_senc_key "secret").
